src/BBConst.v
@@ -1,0 +1,56 @@
+
+From Coq Require Import ZArith List.
+From mathcomp Require Import ssreflect ssrbool ssrnat eqtype seq ssrfun.
+From BitBlasting Require Import Var QFBV CNF BBCommon.
+From ssrlib Require Import ZAriths Tactics.
+From nbits Require Import NBits.
+
+Set Implicit Arguments.
+Unset Strict Implicit.
+Import Prenex Implicits.
+
+
+
+(* ===== bit_blast_const ===== *)
+
+Definition bit_blast_const g (bs : bits) : generator * cnf * word :=
+  (g, [::], map lit_of_bool bs).
+
+Definition mk_env_const E g (bs : bits) : env * generator * cnf * word :=
+  (E, g, [::], map lit_of_bool bs).
+
+Lemma bit_blast_const_correct g bs E g' cs ls :
+  bit_blast_const g bs = (g', cs, ls) -> interp_cnf E (add_prelude cs) ->
+  enc_bits E ls bs.
+Proof.
+  rewrite /bit_blast_const. case=> _ <- <- Hpre. apply: enc_bits_lit_of_bool.
+  exact: (add_prelude_enc_bit_tt Hpre).
+Qed.
+
+Lemma mk_env_const_is_bit_blast_const E g bs E' g' cs ls :
+  mk_env_const E g bs = (E', g', cs, ls) -> bit_blast_const g bs = (g', cs, ls).
+Proof. rewrite /mk_env_const /bit_blast_const. by case=> _ <- <- <-. Qed.
+
+Lemma mk_env_const_sat E g bs E' g' cs lrs :
+  mk_env_const E g bs = (E', g', cs, lrs) -> interp_cnf E' cs.
+Proof. by case=> <- _ <- _. Qed.
+
+Lemma mk_env_const_preserve E g bs E' g' cs lrs :
+  mk_env_const E g bs = (E', g', cs, lrs) -> env_preserve E E' g.
+Proof. case=> <- _ _ _. exact: env_preserve_refl. Qed.
+
+Lemma mk_env_const_newer_gen E g bs E' g' cs lrs :
+  mk_env_const E g bs = (E', g', cs, lrs) -> (g <=? g')%positive.
+Proof. case=> _ <- _ _. exact: Pos.leb_refl. Qed.
+
+Lemma mk_env_const_newer_res E g bs E' g' cs lrs :
+  mk_env_const E g bs = (E', g', cs, lrs) ->
+  newer_than_lit g lit_tt -> newer_than_lits g' lrs.
+Proof.
+  case=> _ <- _ <- Htt {E E' g' cs lrs}. exact: (newer_than_lits_lit_of_bool _ Htt).
+Qed.
+
+Lemma mk_env_const_newer_cnf E g bs E' g' cs lrs :
+  mk_env_const E g bs = (E', g', cs, lrs) ->
+  newer_than_lit g lit_tt -> newer_than_cnf g' cs.
+Proof. by case => _ <- <- _. Qed.
